src/proof/kubernetes_model/list.v
@@ -1,0 +1,85 @@
+From New.proof Require Import prelude empty_ffi.
+From New.proof.kubernetes_model Require Export inv common.
+
+Section proof.
+Context `{hG: !heapGS Σ} {go_ctx: GoContext}.
+Context `{!kviewG Σ}.
+Context `{!cviewG Σ}.
+Context `{!mono_gsetG types.UID.t Σ}.
+
+Lemma wp_State__objListLocked_Pod γ l phys_state_l phys_state abs_state used_uid namespace:
+  {{{ is_pkg_init apimodel ∗
+      "Hstate_m_addr" ∷ l ↦s[apimodel.State :: "m"] phys_state_l ∗
+      "Hown_phys" ∷ phys_state_l ↦$ phys_state ∗
+      "Hown_abs" ∷ own_kview_auth γ abs_state used_uid ∗
+      "Hphys_abs_rep" ∷ ([∗ map] i; obj ∈ phys_state; abs_state, KObjectV.deepown_i i obj 1)
+  }}}
+    l @ (ptrT.id apimodel.State.id) @ "objListLocked" #"Pod"%go #namespace
+  {{{ sl interfaces pods, RET #sl;
+      sl ↦* interfaces ∗
+      ([∗ list] i;pod ∈ interfaces;pods, KObjectV.deepown_i i (KObjectV.Pod pod) 1) ∗
+      ⌜ KObjectV.Pod <$> pods ≡ₚ (map_to_list (filter
+          (λ kv, kv.1.(KKey.Kind') = "Pod"%go ∧ v1.namespace_matches namespace kv.1.(KKey.Namespace'))
+          abs_state)).*2 ⌝ ∗
+      ⌜ Forall PodV.valid pods ⌝ ∗
+      l ↦s[apimodel.State :: "m"] phys_state_l ∗
+      phys_state_l ↦$ phys_state ∗
+      own_kview_auth γ abs_state used_uid ∗
+      ([∗ map] i; obj ∈ phys_state; abs_state, KObjectV.deepown_i i obj 1)
+  }}}.
+Proof.
+Admitted.
+
+Lemma wp_State__objListLocked_Pod_NamespaceAll γ l phys_state_l phys_state abs_state used_uid :
+  {{{ is_pkg_init apimodel ∗
+      "Hstate_m_addr" ∷ l ↦s[apimodel.State :: "m"] phys_state_l ∗
+      "Hown_phys" ∷ phys_state_l ↦$ phys_state ∗
+      "Hown_abs" ∷ own_kview_auth γ abs_state used_uid ∗
+      "Hphys_abs_rep" ∷ ([∗ map] i; obj ∈ phys_state; abs_state, KObjectV.deepown_i i obj 1)
+  }}}
+    l @ (ptrT.id apimodel.State.id) @ "objListLocked" #"Pod"%go #v1.NamespaceAll
+  {{{ sl interfaces pods, RET #sl;
+      sl ↦* interfaces ∗
+      ([∗ list] i;pod ∈ interfaces;pods, KObjectV.deepown_i i (KObjectV.Pod pod) 1) ∗
+      ⌜ KObjectV.Pod <$> pods ≡ₚ (map_to_list (filter (λ kv, kv.1.(KKey.Kind') = "Pod"%go) abs_state)).*2 ⌝ ∗
+      ⌜ Forall PodV.valid pods ⌝ ∗
+      l ↦s[apimodel.State :: "m"] phys_state_l ∗
+      phys_state_l ↦$ phys_state ∗
+      own_kview_auth γ abs_state used_uid ∗
+      ([∗ map] i; obj ∈ phys_state; abs_state, KObjectV.deepown_i i obj 1)
+  }}}.
+Proof.
+  iIntros (Φ) "(#Hinit & Hstate_m_addr & Hown_phys & Hown_abs & Hphys_abs_rep) HΦ".
+  wp_apply (wp_State__objListLocked_Pod with "[$Hstate_m_addr $Hown_phys $Hown_abs $Hphys_abs_rep]").
+  iIntros (sl interfaces pods)
+    "(Hsl & Hlist & %Hperm & %Hpods_valid & Hstate_m_addr & Hown_phys & Hown_abs & Hphys_abs_rep)".
+  iApply "HΦ". iFrame.
+  iPureIntro.
+  assert (filter
+    (λ kv, kv.1.(KKey.Kind') = "Pod"%go ∧
+      v1.namespace_matches v1.NamespaceAll kv.1.(KKey.Namespace')) abs_state =
+    filter (λ kv, kv.1.(KKey.Kind') = "Pod"%go) abs_state) as Hfilter_eq.
+  { apply map_eq. intros k.
+    destruct (abs_state !! k) as [obj|] eqn:Hlookup.
+    - destruct (decide (k.(KKey.Kind') = "Pod"%go)) as [Hkind|Hkind].
+      + transitivity (Some obj).
+        * apply map_lookup_filter_Some_2; [done|].
+          split; [done|left; done].
+        * symmetry. apply map_lookup_filter_Some_2; [done|].
+          done.
+      + transitivity (@None KObjectV.t).
+        * apply map_lookup_filter_None_2. right.
+          intros x Hlookup' [Hkind' _].
+          apply Hkind. exact Hkind'.
+        * symmetry. apply map_lookup_filter_None_2. right.
+          intros x Hlookup' Hpred.
+          apply Hkind. exact Hpred.
+    - transitivity (@None KObjectV.t).
+      + apply map_lookup_filter_None_2. left. done.
+      + symmetry. apply map_lookup_filter_None_2. left. done.
+  }
+  rewrite Hfilter_eq in Hperm.
+  split; [exact Hperm|exact Hpods_valid].
+Qed.
+
+End proof.
